@prefix edehmap: <http://purl.org/edeh/mappingPredicates#> .
@prefix dcterms: <http://purl.org/dc/terms/> .
@prefix desm: <https://desmsolutions.org/ns/> .
@prefix skos: <http://www.w3.org/2004/02/skos/core#> .
@prefix xsd: <http://www.w3.org/2001/XMLSchema#> .

<http://purl.org/edeh/mappingPredicates> a skos:ConceptScheme ;
    dcterms:created "2026-01-24"^^xsd:date ;
    dcterms:creator "EDEH Task Force 2"@en ;
    dcterms:description "This concept scheme identifies the mapping predicates used for DESM."@en ;
    dcterms:title "EDEH Mapping Predicates"@en ;
    skos:hasTopConcept
        edehmap:identical ,
        edehmap:similar ,
        edehmap:aggregated ,
        edehmap:disaggregated ,
        edehmap:concept ,
        edehmap:noMatch .

edehmap:identical a skos:Concept ;
    skos:definition "The definition is identical in intent, with identical wording or minor differences."@en ;
    skos:inScheme <http://purl.org/edeh/mappingPredicates> ;
    skos:prefLabel "Identical"@en ;
    desm:weight 5 .

edehmap:similar a skos:Concept ;
    skos:definition "The definition is similar in intent, but with wording differences."@en ;
    skos:inScheme <http://purl.org/edeh/mappingPredicates> ;
    skos:prefLabel "Similar"@en ;
    desm:weight 4 .

edehmap:aggregated a skos:Concept ;
    skos:definition "Single property in the spine maps to multiple properties in the specification being mapped."@en ;
    skos:inScheme <http://purl.org/edeh/mappingPredicates> ;
    skos:prefLabel "Aggregated"@en ;
    desm:weight 3 .

edehmap:disaggregated a skos:Concept ;
    skos:definition "Multiple properties in the spine, map to the property in the specification being mapped."@en ;
    skos:inScheme <http://purl.org/edeh/mappingPredicates> ;
    skos:prefLabel "Disaggregated"@en ;
    desm:weight 3 .

edehmap:concept a skos:Concept ;
    skos:definition "The definition is related only at a conceptual level, with differences in the intention."@en ;
    skos:inScheme <http://purl.org/edeh/mappingPredicates> ;
    skos:prefLabel "Concept"@en ;
    desm:weight 2 .

edehmap:issue a skos:Concept ;
    skos:definition "Annotation to explain alignment where necessary to clarify or to interpret the mapping."@en ;
    skos:inScheme <http://purl.org/edeh/mappingPredicates> ;
    skos:prefLabel "Issue"@en ;
    desm:weight 1 .

edehmap:noMatch a skos:Concept ;
    skos:definition "There's no property to match to the property of a class in the spine."@en ;
    skos:inScheme <http://purl.org/edeh/mappingPredicates> ;
    skos:prefLabel "No Match"@en ;
    desm:weight 0 .

